Prove reflection for compilers, mod well-foundedness for term_ok reflection

src/named/PfCompilers.v
@@ -99,12 +99,14 @@ Inductive preserving_compiler (target : pf_lang) : compiler -> pf_lang -> Prop :
     (*is_exp t ->should I have this here? prob. not*)
     preserving_compiler target ((n, e)::cmp) ((n,term_rule_pf c args t) :: l)
 | preserving_compiler_sort_le : forall cmp l n c teq t1 t2,
+    preserving_compiler target cmp l ->
     (* Notable: only uses the previous parts of the compiler on c *)
     sort_ok target (compile_ctx l cmp c) teq ->
     compile l cmp t1 = proj_l target teq ->
     compile l cmp t2 = proj_r target teq ->
     preserving_compiler target ((n,teq)::cmp) ((n,sort_le_pf c t1 t2) :: l)
 | preserving_compiler_term_le : forall cmp l n c eeq e1 e2 t,
+    preserving_compiler target cmp l ->
     (* Notable: only uses the previous parts of the compiler on c *)
     term_ok target (compile_ctx l cmp c) eeq (compile l cmp t) ->
     compile l cmp e1 = proj_l target eeq ->
@@ -140,16 +142,54 @@ Fixpoint check_preserving tgt (cmp:compiler) src : bool :=
   | _, _ => false
   end.
 
+
+Lemma fresh_compile_ctx x s cmp c
+  : fresh x c -> fresh x (compile_ctx s cmp c).
+Proof.
+  induction c; break; simpl in *; intros; break; break_goal; auto.
+  rewrite in_cons.
+  rewrite in_cons in H.
+  apply /norP;
+    move: H => /norP H;
+  break; break_goal; auto.
+Qed.
+
+
+Lemma all_fresh_compile_ctx s cmp c
+  : all_fresh c -> all_fresh (compile_ctx s cmp c).
+Proof.
+  induction c; break; simpl in *;
+    intros; break; break_goal;auto;
+      apply fresh_compile_ctx; assumption.
+Qed.
+Hint Resolve all_fresh_compile_ctx : pfcore.
+
+(*TODO: move to utils; separate db?*)
+Lemma false_False : false -> False.
+Proof.
+  intro h; inversion h.
+Qed.
+Hint Resolve false_False : pfcore.
+  
 Lemma check_preservingP
-  : forall t cmp s, check_lang_ok s ->
+  : forall t cmp s, all_fresh t ->
+                    check_lang_ok s ->
     reflect (preserving_compiler t cmp s) (check_preserving t cmp s).
 Proof.
-  intros t cmp; induction cmp; intros s sok; destruct s; break;
-   repeat (simpl in *; break;lazymatch goal with
+  Opaque all_fresh.
+  intros t cmp; induction cmp; intros s frt sok; destruct s; break;
+   repeat (simpl in *; break;(lazymatch goal with
+    | [H: ?a |- ?a] => exact H
     | [H: true = true |- _] => clear H
-    | [H: (_ == _) = true |- _] => move: H => /eqP; intro H; subst
     | [H: true = _ |- _] => symmetry in H
     | [H: false = true|- _] => inversion H
+    | [H: false = _ |- _] => symmetry in H
+    | [H: is_true false|- _] => inversion H
+    | [H: ?a = true |- _] => change (is_true a) in H
+    | [H: (?a == ?a) = false|- _] => rewrite eq_refl in H
+    | [H: (?a == ?b) = false,
+       H' : ?a = ?b |- _] => exfalso; move: H => /negP H; apply H; apply /eqP; exact H'
+    | [H: is_true(_ == _) |- _] => move: H => /eqP; intro H; subst
     | [|- reflect _ true] => constructor
     | [|- reflect _ false] => constructor
     | [|- reflect _ (match ?e with _=>_ end)] => destruct e
@@ -158,790 +198,42 @@ Proof.
     | [|- reflect _ ?p] =>
       let eqn := fresh "eqn" in
       my_case eqn p; simpl
-    | [IH : forall _, _ -> reflect (preserving_compiler _ _ _) _,
-       H : check_preserving ?t ?c ?s = true |- preserving_compiler ?t ?c ?s] =>
+    | [H' : is_true(all_fresh ?l) -> ?a |- _] =>
+      assert a; [apply H'|]; clear H'
+    | [IH : forall _, _ -> _ -> reflect (preserving_compiler _ _ _) _,
+       H : is_true(check_preserving ?t ?c ?s) |- preserving_compiler ?t ?c ?s] =>
       apply /IH; auto
     | [|- preserving_compiler _ _ _] => constructor
-    | [H : check_sort_ok ?t ?c ?s = true |- sort_ok ?t ?c ?s] =>
-      apply /sort_okP; auto
-    | [|- ~_] => let H:= fresh in intro H; inversion H; subst; clear H 
-          end).
-
-  Lemma check_ctx_okP.
-  Lemma ctx_ok_all_fresh
-  simpl in sok0.
-  match goal with
-    
-    | [H : check_sort_ok ?t ?c ?s = true |- sort_ok ?t ?c ?s] =>
+    | [H : check_preserving ?t ?cmp ?s = false,
+       H' : preserving_compiler ?t ?cmp ?s|- _]=>
+      move: H' => /IHcmp; rewrite H; auto
+    | [H : is_true(check_sort_ok ?t ?c ?s) |- sort_ok ?t ?c ?s] =>
       apply /check_sort_okP; auto
-  end.
-  constructor.
-  repeat rewrite -?Bool.andb_assoc.
-  Unset Printing Notations.
-  TODO: handle and
-  {
-    
-  Search _ (_&&_&&_).
-(*
-
-Lemma wf_empty_sort c t : ~wf_sort [::] c t.
-Proof using .
-  by inversion.
+    | [|- is_exp _]=> apply /check_is_expP; auto
+    | [|- ~_] => let H:= fresh in intro H; inversion H; subst; clear H 
+    | [H : check_term_ok _ _ ?e ?t = false, H' : term_ok _ _ ?e ?t|- _]=>
+      move: H' => /check_term_okP; rewrite H; auto
+    | [H : check_sort_ok _ _ ?t = false, H' : sort_ok _ _ ?t|- _]=>
+      move: H' => /check_sort_okP; rewrite H; auto
+    | [H : check_ctx_ok _ _ = false, H' : ctx_ok _ _|- _]=>
+      move: H' => /check_ctx_okP; rewrite H; auto
+    | [H : check_rule_ok _ _ = false, H' : rule_ok _ _|- _]=>
+      move: H' => /check_rule_okP; rewrite H; auto
+    | [H : check_is_exp ?e = false, H' : is_exp ?e|- _]=>
+      move: H' => /check_is_expP; rewrite H; auto
+    | [H : is_true(check_term_ok _ _ _ _)|- _]=>
+      move: H => /check_term_okP H
+    | [H : is_true(check_ctx_ok _ _)|- _]=>
+      move: H => /check_ctx_okP H
+    | [H : is_true(check_lang_ok _)|- _]=>
+      move: H => /check_lang_okP H
+    | [|- is_true(all_fresh (compile_ctx _ _ _))] =>
+      apply all_fresh_compile_ctx
+    | [H : ctx_ok ?l ?c |- is_true(all_fresh ?c)] =>
+      apply (ctx_ok_all_fresh H)
+    | [H : lang_ok ?l |- is_true(all_fresh ?l)] =>
+      apply lang_ok_all_fresh
+    | [|- _ -> False] => intro
+    end ||
+        match goal with [|-?P] => idtac P end)).
 Qed.
-
-Lemma wf_empty_ctx c : wf_ctx [::] c -> c = [::].
-Proof using .
-  case; auto.
-  intros.
-  exfalso.
-  eapply wf_empty_sort; eassumption.
-Qed.
-
-(*
-Lemma wf_empty_term c e t : wf_ctx [::] c -> ~wf_term [::] c e t.
-Proof using .
-  intros wfc wft.
-  elim: wft wfc; eauto.
-  intros n t0 nin.
-  move /wf_empty_ctx => wfe.
-  move: wfe nin => ->.
-  auto.  
-Qed.
-*)
-
-(*TODO: move to core*)
-
-Lemma with_names_from_nil_r (c : ctx) : with_names_from c (@nil exp) = [::].
-Proof.
-  case: c; simpl; auto; case; auto.
-Qed.
-
-
-
-Ltac f_equal_match :=
-  match goal with
-  | [|- match ?e with _ => _ end = match ?e with _ => _ end]
-    => let e':= fresh in remember e as e'; destruct e'
-  end.
-
-(*
-Lemma lookup_in_tail c c' n t s s'
-    : let cs' := with_names_from (c'++ c) (s' ++ s) in
-    size s == size c ->
-    size s' == size c' ->
-    all_fresh (c' ++ c) ->
-    (n,t) \in c ->
-              named_list_lookup (var n) cs' n =
-              named_list_lookup (var n) (with_names_from c s) n.
-Proof.
-  simpl.
-  elim: c' s'.
-  {
-    case; simpl; auto.
-    intros a l _.
-    move /eqP; inversion.
-  }
-  {
-    intros until s'.
-    case: s'.
-    {
-      intro b.
-      move /eqP; inversion.
-    }
-    {
-      destruct a.
-      intros e s' szeq.
-      simpl; move /eqP; case; move /eqP => szeq'.
-      move /andP => [fs0 nlaf] nin.
-      suff: ((n=?s0)%string = false); [move ->; eauto|].
-      admit.
-    }
-  }
-Admitted.
-*)
-
-Lemma fresh_compile_ctx c cmp n
-  : fresh n c -> fresh n (compile_ctx cmp c).
-Proof using.
-  elim: c; simpl; auto.
-  move => [n' t] c'.
-  unfold fresh.
-  intro IH; simpl.
-  rewrite !in_cons.
-  move /norP => [nneq nnin].
-  apply /norP.
-  split; auto.
-Qed.
-
-Local Ltac in_preserving_sort_rec :=
-  intros;
-      match goal with
-        [ Hin : is_true(_\in_),
-          IH : is_true(_\in_) -> exists t,_ |- _] =>
-        move: (IH Hin); case; intros
-      end; solve [eauto 3 | eexists; rewrite in_cons; apply /orP; eauto].
-
-Lemma in_preserving_sort lt cmp ls n c' args
-  : preserving_compiler lt cmp ls ->
-    (n, sort_rule c' args) \in ls ->
-    exists t,(n, sort_case (map fst c') t) \in cmp.
-Proof using .
-  elim; simpl; eauto; intros;
-    try  match goal with
-    [ H : is_true(_\in_::_)|- _] =>
-    revert H; rewrite in_cons; move /orP; case
-    end; try solve [move/eqP; case; done| in_preserving_sort_rec].
-  { 
-    move /eqP => [neq ceq].
-    subst.
-    exists t.
-    rewrite in_cons.
-    apply /orP.
-    left.
-    apply /eqP; reflexivity.
-  }
-  Unshelve.
-  exact (scon "ERR" [::]).
-Qed.
-
-Lemma in_preserving_term lt cmp ls n c' args t
-  : preserving_compiler lt cmp ls ->
-    (n, term_rule c' args t) \in ls ->
-    exists e,(n, term_case (map fst c') e) \in cmp.
-Proof using .
-  elim; simpl; eauto; intros;
-    try  match goal with
-    [ H : is_true(_\in_::_)|- _] =>
-    revert H; rewrite in_cons; move /orP; case
-    end; try solve [move/eqP; case; done| in_preserving_sort_rec].
-  { 
-    move /eqP => [neq ceq teq].
-    subst.
-    exists e.
-    rewrite in_cons.
-    apply /orP.
-    left.
-    apply /eqP; reflexivity.
-  }
-  Unshelve.
-  exact (con "ERR" [::]).
-Qed.
-
-Lemma named_list_all_fresh_lookup {A : eqType} l n (e default : A)
-  : all_fresh l ->
-    (n, e) \in l ->
-    named_list_lookup default l n = e.
-Proof using .
-  elim: l; [ by cbv |].
-  move => [n' e'] l IH; simpl.
-  move /andP => [ fn allf].
-  rewrite in_cons.
-  case neq: (n == n').
-  case eeq: (e == e').
-  {
-    move: neq eeq => /eqP neq /eqP eeq.
-    rewrite -!neq -!eeq.
-    move /orP; case; intros; subst;
-    rewrite eqb_refl; reflexivity.
-  }
-  {
-    pose neq' := neq.
-    cbn.
-    cbn in neq.
-    rewrite neq.
-    rewrite eeq.
-    simpl.
-    clear IH.
-    move: neq' fn => /eqP ->.
-    intros.
-    exfalso.
-    pose p := (fresh_neq_in fn H).
-    move: p.
-    move /eqP.
-    done.
-  }
-  {
-    suff: ((n, e) == (n', e') = false); [ move ->; simpl|].
-    2:{
-      rewrite -Bool.negb_true_iff.
-      apply /negP.
-      move /eqP.
-      case.
-      move /eqP.
-      by rewrite neq.
-    }
-    pose p := neq; cbn in p; rewrite p; clear p.
-    auto.
-  } 
-Qed.
-
-Lemma preserving_compiler_fresh n lt cmp ls
-  : preserving_compiler lt cmp ls ->
-    fresh n ls ->
-    fresh n cmp.
-Proof using .
-  elim; simpl; auto; solve
-  [unfold fresh; intro_to is_true;
-  simpl;
-  rewrite !in_cons !negb_or; simpl;
-  move /andP; case; intros; try apply /andP; auto].
-Qed.
-
-  
-Lemma preserving_compiler_all_fresh lt cmp ls
-  : preserving_compiler lt cmp ls ->
-    all_fresh ls ->
-    all_fresh cmp.
-Proof using .
-  elim; simpl; auto; intro_to is_true;
-    move /andP => [frn af]; auto; apply /andP; split; auto.
-  all: eapply preserving_compiler_fresh;eauto.
-Qed. 
-Hint Resolve preserving_compiler_all_fresh : judgment.
-
-(* TODO: move to Core *)
-Lemma wf_lang_all_fresh l : wf_lang l -> all_fresh l.
-Proof.
-  elim; intros; simpl in *; auto.
-  apply /andP; auto.
-Qed.
-Hint Resolve wf_lang_all_fresh : judgment.
-
-
-Lemma term_fresh_strengthen n cc l cmp c e t
-  : fresh n l ->
-    wf_term l c e t ->
-    compile_term ((n, cc) :: cmp) e = compile_term cmp e
-with args_fresh_strengthen n cc l cmp c s args es c'
-  : fresh n l ->
-    wf_args l c s args es c' ->
-    compile_args ((n, cc) :: cmp) s = compile_args cmp s.
-Proof using .
-  {
-    intro_to wf_term; inversion; subst; simpl in *; eauto.
-    {
-      suff: ((n0 =? n)%string = false);[ move ->|].
-      {
-        f_equal_match; auto.
-        change (map (compile_term ?cmp)) with (compile_args cmp).
-        erewrite args_fresh_strengthen; eauto.
-      }
-      {
-        apply /negP.
-        apply /negP.
-        eapply fresh_neq_in; eauto.
-      }
-    }
-  }
-  {
-    intro_to wf_args; inversion; subst; simpl in *; eauto.
-    f_equal; eauto.
-  }    
-Qed.    
-    
-Lemma sort_fresh_strengthen n cc l cmp c t
-  : fresh n l ->
-    wf_sort l c t ->
-    compile_sort ((n, cc) :: cmp) t = compile_sort cmp t.
-Proof using .
-  intro_to wf_sort; inversion; subst.
-  simpl.
-  suff: ((n0 =? n)%string = false);[ move ->|].
-  {
-    f_equal_match; auto.
-    erewrite args_fresh_strengthen; eauto.
-  }
-  {
-    apply /negP.
-    apply /negP.
-    eapply fresh_neq_in; eauto.
-  }
-Qed.
-  
-Lemma ctx_fresh_strengthen n cc l cmp c
-  : fresh n l ->
-    wf_ctx l c ->
-    compile_ctx ((n, cc) :: cmp) c = compile_ctx cmp c.
-Proof.
-  elim: c; simpl; auto.
-  intro_to wf_ctx; inversion; subst.
-  simpl.
-  f_equal; auto.
-  erewrite sort_fresh_strengthen; eauto.
-Qed.  
-
-
-(*TODO:move to Core*)
-(* TODO:add hints?
-(* a hint for a common case*)
-Lemma wf_ctx_from_sort_rule_in l c n
-  : wf_lang l -> (n, sort_rule c) \in l -> wf_ctx l c.
-Proof.
-  intros wfl cin; apply rule_in_wf in cin; inversion cin; done.
-Qed.
-Hint Resolve wf_ctx_from_sort_rule_in : judgment.
-(* a hint for a common case*)
-Lemma wf_ctx_from_term_rule_in l c t n
-  : wf_lang l -> (n, term_rule c t) \in l -> wf_ctx l c.
-Proof.
-  intros wfl cin; apply rule_in_wf in cin; inversion cin; done.
-Qed.
-Hint Resolve wf_ctx_from_term_rule_in : judgment.
-(* a hint for a common case*)
-Lemma wf_sort_from_term_rule_in l c t n
-  : wf_lang l -> (n, term_rule c t) \in l -> wf_sort l c t.
-Proof.
-  intros wfl cin; apply rule_in_wf in cin; inversion cin; done.
-Qed.
-Hint Resolve wf_sort_from_term_rule_in : judgment.
-*)
-
-(* TODO: move to utils*)
-(* decomposes the way you want \in to on all_fresh lists*)
-Fixpoint in_once {A:eqType} n e (l : named_list A) : bool :=
-  match l with
-  | [::] => false
-  | (n',e')::l' =>
-    ((n == n') && (e == e')) || ((n != n')&&(in_once n e l'))
-  end.
-
-Arguments in_once {A} n e !l/.
-
-Lemma in_once_notin {A:eqType} n (e : A) l
-  : n \notin (map fst l) -> ~~(in_once n e l).
-Proof using .
-  elim: l; auto; intros; break; simpl in *.
-  rewrite ?in_cons in H0.
-  move: H0.
-  case neq: (n==s); auto.
-Qed.
-
-Lemma all_fresh_in_once {A:eqType} n (e : A) l
-  : all_fresh l -> ((n,e) \in l) = in_once n e l.
-Proof using .
-  elim: l; simpl; auto; intros; repeat (break; simpl in * ).
-  rewrite in_cons.
-  rewrite H; auto.
-  change ((n,e)==(s,s0)) with ((n==s)&&(e==s0)).
-  case neq: (n == s); simpl; auto.
-  rewrite Bool.orb_false_r.
-  case eeq:(e==s0); simpl; auto.
-  apply /negP.
-  apply /negP.
-  move: neq => /eqP ->.
-  by apply in_once_notin.
-Qed.  
-
-
-Local Ltac setup_inv_lem :=
-  let pc := fresh "pc" in
-  let wfl := fresh "wfl" in
-  let frls := fresh "frls" in
-  let frcmp := fresh "frcmp" in
-  intros pc wfl;
-  suff: all_fresh ls; eauto with judgment;  intro frls;
-  suff: all_fresh cmp; eauto with judgment; intro frcmp;
-  rewrite !all_fresh_in_once; auto;
-  revert pc wfl frls frcmp.
-
-
-(* TODO: relate independent judgment to elab
-   to port core lemmas.
-*)
-Parameter rule_in_wf
-     : forall (l : lang) (r : rule) (n : string),
-       wf_lang l -> (n, r) \in l -> wf_rule l r.
-
-Local Ltac inv_lem_step :=
-  match goal with
-  | H : wf_lang (_::_)|-_=> inversion H; subst; clear H
-  | H : wf_rule _ _|-_=>inversion H; subst; clear H
-  | H : is_true(_ || _) |- _=> move: H => /orP; case => H; break
-  | H : is_true(_ == _) |- _=> move: H => /eqP; (try by inversion); repeat case; intros; subst
-  | H : is_true(?a != ?a) |- _=> by rewrite eq_refl in H
-  | H : is_true(in_once _ _ _) |- wf_ctx _ _ =>
-    rewrite -all_fresh_in_once in H; auto; apply rule_in_wf in H; inversion H; subst; eassumption
-  | H : is_true(in_once _ _ _) |- wf_sort _ _ _ =>
-    rewrite -all_fresh_in_once in H; auto; apply rule_in_wf in H; inversion H; subst; eassumption
-  | H : is_true(in_once _ _ _) |- wf_term _ _ _ _ =>
-    rewrite -all_fresh_in_once in H; auto; apply rule_in_wf in H; inversion H; subst; eassumption
-  | |- context[ compile_ctx (_::_) _] => erewrite ctx_fresh_strengthen; eauto with judgment
-  | |- context[ compile_sort (_::_) _] => erewrite sort_fresh_strengthen; eauto with judgment
-  | |- context[ compile_term (_::_) _] => erewrite term_fresh_strengthen; eauto with judgment
-  end.
-
-Local Ltac prove_inv_lem :=
-  setup_inv_lem;
-  elim; [by cbv|..];
-    intros; simpl in *; break;
-  repeat inv_lem_step; eauto.
-
-Lemma preserving_sort_case_inv n t c args lt cmp ls
-  :  preserving_compiler lt cmp ls ->
-     wf_lang ls ->
-     (n, sort_rule c args) \in ls ->
-     (n, sort_case args t) \in cmp ->
-     wf_sort lt (compile_ctx cmp c) t.
-Proof using . prove_inv_lem. Qed.
-
-Lemma preserving_term_case_inv n t e c args lt cmp ls
-  :  preserving_compiler lt cmp ls ->
-     wf_lang ls ->
-     (n, term_rule c args t) \in ls ->
-     (n, term_case args e) \in cmp ->
-     wf_term lt (compile_ctx cmp c) e (compile_sort cmp t).
-Proof using . prove_inv_lem. Qed.
-
-
-Lemma preserving_sort_le_inv n t1 t2 c lt cmp ls
-  :  preserving_compiler lt cmp ls ->
-     wf_lang ls ->
-     (n, sort_le c t1 t2) \in ls ->
-     le_sort lt (compile_ctx cmp c) (compile_sort cmp t1) (compile_sort cmp t2).
-Proof using . prove_inv_lem. Qed.
-
-Lemma preserving_term_le_inv n t e1 e2 c lt cmp ls
-  :  preserving_compiler lt cmp ls ->
-     wf_lang ls ->
-     (n, term_le c e1 e2 t) \in ls ->
-     le_term lt (compile_ctx cmp c) (compile_sort cmp t) (compile_term cmp e1) (compile_term cmp e2).
-Proof using . prove_inv_lem. Qed.
-
-
-Lemma f_apply_case_map {A B} (f : A -> B) cc b1 b2
-  : f match cc with
-      | sort_case args c_case => b1 args c_case
-      | term_case args c_case => b2 args c_case
-      end
-    = match cc with
-      | sort_case args c_case => f (b1 args c_case)
-      | term_case args c_case => f (b2 args c_case)
-      end.
-Proof.
-  case: cc; reflexivity.
-Qed.
-
-
-Lemma subst_zip args s s'
-  : (zip args s)[/s'/] = zip args s[/s'/].
-Proof.
-  elim: args s; intros until s; case: s; intros; break; simpl in *; auto.
-  f_equal.
-  by fold_Substable.
-Qed.
-
-
-(* TODO: finish these
-Lemma compile_subst_lookup s n cmp
-  : compile_term cmp (subst_lookup s n) = subst_lookup (compile_subst cmp s) n.
-Proof.
-  elim: s; intros; break; simpl in *; auto.
-  change (?n =? ?s)%string with (n==s).
-  case neq: (n == s); simpl in *; auto.
-Qed.
-
-Lemma compile_term_subst cmp e s
-  : well_scoped (map fst s) e -> compile_term cmp (e[/s/]) = (compile_term cmp e)[/compile_subst cmp s/]
-with compile_args_subst cmp e s
-  : well_scoped (map fst s) e -> compile_args cmp (e[/s/]) = (compile_args cmp e)[/compile_subst cmp s/].
-Proof.
-  {
-    case: e; intros; simpl in *; auto using compile_subst_lookup.
-    case_match; simpl; auto.
-    rewrite subst_assoc; fold_Substable.
-    {
-      rewrite subst_zip.
-      unfold compile_args in *.
-      by rewrite compile_args_subst.
-    }
-    {
-      Search _ (map _ (zip _ _)).
-(* TODO: ws assumption; need ws_compiler
- *)
-Admitted.
-Proof.
-  (* TODO: requires induction *)
-Admitted.
-
-Lemma compile_sort_subst cmp t s
-  : compile_sort cmp (t[/s/]) = (compile_sort cmp t)[/compile_subst cmp s/].
-Proof.
-  case: t; simpl.
-  intros n a.
-  case_match; simpl; auto.
-  rewrite subst_assoc.
-  fold_Substable.
-  rewrite subst_zip.
-  Lemma subst_zip
-    : (zip args s)[/s'/] = zip args s[/s'/].
-  rewrite (f_apply_case_map (sort_subst (compile_subst cmp s))).
-  f_equal_match; simpl; auto.
-Admitted.
-
-
-
-
-Lemma with_names_from_zip c s
-  : with_names_from c s = zip (map fst c) s.
-Proof.
-  elim: c s; [| case]; intros until s; case: s; simpl; auto.
-  intros.
-  f_equal.
-  eauto.
-Qed.
-
-
-Lemma compile_with_names_from cmp c s
-  : compile_subst cmp (with_names_from c s)
-    = with_names_from c (map (compile_term cmp) s).
-Proof.
-  elim: c s; [| case]; intros until s; case: s; simpl; auto.
-  intros.
-  f_equal.
-  eauto.
-Qed.
-
-
-Lemma compile_ctx_in cmp n t c
-  : (n,t) \in c -> (n, compile_sort cmp t) \in compile_ctx cmp c.
-Proof.
-  elim: c; simpl; auto.
-  case; intro_to is_true.
-  rewrite in_cons.
-  move /orP; case.
-  {
-    move /eqP; case; intros; subst.
-    rewrite in_cons.
-    apply /orP; left.
-    apply /eqP; f_equal.
-  }
-  {
-    simpl.
-    intro.
-    rewrite in_cons.
-    apply /orP; auto.
-  }
-Qed.
-
-
-Lemma compile_ctx_fst c cmp : map fst (compile_ctx cmp c) = map fst c.
-Proof.
-  elim: c; auto.
-  case => n s l //= -> //.
-Qed.
-
-Lemma inductive_implies_semantic_sort_wf cmp ls lt
-  : wf_lang ls -> wf_lang lt -> preserving_compiler lt cmp ls ->
-    sort_wf_preserving_sem cmp ls lt
-with inductive_implies_semantic_term_wf cmp ls lt
-  : wf_lang ls -> wf_lang lt -> preserving_compiler lt cmp ls ->
-    term_wf_preserving_sem cmp ls lt
-with inductive_implies_semantic_args_wf cmp ls lt
-  : wf_lang ls -> wf_lang lt -> preserving_compiler lt cmp ls ->
-    args_wf_preserving_sem cmp ls lt
-with inductive_implies_semantic_ctx_wf cmp ls lt
-  : wf_lang ls -> wf_lang lt -> preserving_compiler lt cmp ls ->
-    ctx_wf_preserving_sem cmp ls lt
-with inductive_implies_semantic_sort_le cmp ls lt
-  : wf_lang ls -> wf_lang lt -> preserving_compiler lt cmp ls ->
-    sort_le_preserving_sem cmp ls lt
-with inductive_implies_semantic_term_le cmp ls lt
-  : wf_lang ls -> wf_lang lt -> preserving_compiler lt cmp ls ->
-    term_le_preserving_sem cmp ls lt
-with inductive_implies_semantic_args_le cmp ls lt
-  : wf_lang ls -> wf_lang lt -> preserving_compiler lt cmp ls ->
-    args_le_preserving_sem cmp ls lt.
-Proof.
-  all: intros wfs wft pc c.
-  {
-    intros t.    
-    case; intros; simpl.
-    pose in_cmp := i; eapply in_preserving_sort in in_cmp; destruct in_cmp as [e H]; eauto.
-    erewrite named_list_all_fresh_lookup; eauto using preserving_compiler_fresh.
-    simpl.
-    eapply mono_subst_wf_sort; auto. 
-    { eapply preserving_sort_case_inv; eauto. }
-    {
-      eapply inductive_implies_semantic_ctx_wf; [| |eauto |]; eauto with judgment.
-    }
-    {
-      replace (map fst c') with (map fst (compile_ctx cmp c')).
-      apply wf_subst_from_wf_args.
-      eapply inductive_implies_semantic_args_wf;  [| |eauto |]; eauto with judgment.
-      admit(* TODO: lemma*).
-    }
-    {
-      eauto using preserving_compiler_all_fresh, wf_lang_all_fresh.
-    }
-  }
-  {
-    intros e t.
-    case; intros; simpl.
-    {
-       pose in_cmp := i; eapply in_preserving_term in in_cmp; destruct in_cmp as [e' H]; eauto.
-       erewrite named_list_all_fresh_lookup; eauto using preserving_compiler_fresh.
-       simpl.
-       rewrite compile_sort_subst.
-       rewrite -with_names_from_zip.
-       rewrite -compile_with_names_from.
-       eapply mono_subst_wf_term; eauto. 
-       { admit (*TODO: term version eapply preserving_sort_case_inv; eauto.*). }
-       {
-         eapply inductive_implies_semantic_ctx_wf; [| |eauto |]; eauto.
-         apply rule_in_wf in i; auto.
-         inversion i; subst; eauto.
-       }
-       {
-         admit(*
-         rewrite compile_subst_compile_args.
-         apply wf_subst_from_wf_args.
-         eapply inductive_implies_semantic_args_wf;  [| |eauto |]; eauto with judgment.
-         admitTODO: lemma*).
-       }
-       {
-         eauto using preserving_compiler_all_fresh, wf_lang_all_fresh.
-       }
-    }
-    {
-      eapply wf_term_conv.
-      { eapply inductive_implies_semantic_sort_wf; [| |eauto |]; eauto. }
-      { eapply inductive_implies_semantic_term_wf; [| |eauto |]; eauto. }
-      { eapply inductive_implies_semantic_sort_le; [| |eauto |]; eauto. }
-    }
-    {
-      constructor; eauto.
-      by apply compile_ctx_in.
-    }
-  }
-  {
-    intro_to wf_args; case; simpl; constructor.
-    { by apply fresh_compile_ctx. }
-    { eapply inductive_implies_semantic_args_wf; [| |eauto |]; eauto. }
-    { eapply inductive_implies_semantic_sort_wf; [| |eauto |]; eauto. }
-    {
-      rewrite -compile_with_names_from.
-      rewrite -compile_sort_subst.
-      eapply inductive_implies_semantic_term_wf; [| |eauto |]; eauto.
-      rewrite with_names_from_zip.
-      rewrite compile_ctx_fst.
-      rewrite -with_names_from_zip.
-      done.
-    }
-  }
-  {
-    intro_to wf_ctx; case; simpl; constructor.
-    { by apply fresh_compile_ctx. }
-    { eapply inductive_implies_semantic_ctx_wf; [| |eauto |]; eauto. }
-    { eapply inductive_implies_semantic_sort_wf; [| |eauto |]; eauto. }
-  }
-  {
-    intro_to le_sort; case; simpl; intros.
-    {
-      admit (*TODO: inversion lemma*).
-    }
-    {
-      rewrite !compile_sort_subst.
-      eapply le_sort_subst.
-      { admit (*TODO: le subst,not leargs?
-                eapply inductive_implies_semantic_subst_le; [| |eauto |]; eauto.*). }
-      { eapply inductive_implies_semantic_sort_le; [| |eauto |]; eauto. }
-    }
-    { eapply le_sort_refl. }
-    { eapply le_sort_trans.
-      { eapply inductive_implies_semantic_sort_le; [| |eauto |]; eauto. }
-      { eapply inductive_implies_semantic_sort_le; [| |eauto |]; eauto. }
-    }
-    {
-      eapply le_sort_sym.
-      { eapply inductive_implies_semantic_sort_le; [| |eauto |]; eauto. }
-    }
-  }
-  {
-    intro_to le_term; case; simpl; intros.
-    {
-      rewrite !compile_sort_subst.
-      rewrite !compile_term_subst.
-      eapply le_term_subst.
-      { admit (*TODO: le subst,not leargs?
-                eapply inductive_implies_semantic_subst_le; [| |eauto |]; eauto.*). }
-      { eapply inductive_implies_semantic_term_le; [| |eauto |]; eauto. }
-    }
-    
-    {
-      admit (*TODO: inversion lemma*).
-    }
-    { eapply le_term_refl. }
-    { eapply le_term_trans.
-      { eapply inductive_implies_semantic_term_le; [| |eauto |]; eauto. }
-      { eapply inductive_implies_semantic_term_le; [| |eauto |]; eauto. }
-    }
-    {
-      eapply le_term_sym.
-      { eapply inductive_implies_semantic_term_le; [| |eauto |]; eauto. }
-    }
-    {
-      eapply le_term_conv.
-      { eapply inductive_implies_semantic_sort_le; [| |eauto |]; eauto. }
-      { eapply inductive_implies_semantic_term_le; [| |eauto |]; eauto. }
-    }
-  }
-  {
-    intro_to le_args; case; simpl; intros; constructor.
-    { eapply inductive_implies_semantic_args_le; [| |eauto |]; eauto. }
-    { by apply fresh_compile_ctx. }
-    {
-      rewrite -compile_with_names_from.
-      rewrite -compile_sort_subst.
-      eapply inductive_implies_semantic_term_le; [| |eauto |]; eauto.
-      rewrite with_names_from_zip.
-      rewrite compile_ctx_fst.
-      rewrite -with_names_from_zip.
-      done.
-    }
-  }
-Admitted.
-  
-        
-    
-
-Lemma inductive_implies_semantic cmp ls lt
-  : wf_lang ls -> wf_lang lt ->
-    preserving_compiler lt cmp ls ->
-    semantics_preserving cmp ls lt.
-Proof.
-  intros.
-  repeat split.
-  by eapply inductive_implies_semantic_sort_wf.
-  by eapply inductive_implies_semantic_term_wf.
-  by eapply inductive_implies_semantic_args_wf.
-  by eapply inductive_implies_semantic_sort_le.
-  by eapply inductive_implies_semantic_term_le.
-  by eapply inductive_implies_semantic_args_le.
-Qed.
-
-(*
-Lemma semantic_implies_inductive cmp ls lt
-  : wf_lang ls -> wf_lang lt ->
-    semantics_preserving cmp ls lt ->
-    preserving_compiler lt cmp ls.
-Proof.
-  (* TODO: actually quite non-trivial *)
-*)
-*)
-
-
-Fixpoint make_compiler
-           (cmp_sort : string -> list string -> sort)
-           (cmp_exp : string -> list string -> exp)
-           (l : lang) : compiler :=
-  match l with
-  | (n,sort_rule c args)::l' =>
-    (n,sort_case args (cmp_sort n args))
-      ::(make_compiler cmp_sort cmp_exp l')
-  | (n,term_rule c args _)::l' => (n,term_case args (cmp_exp n args))
-      ::(make_compiler cmp_sort cmp_exp l')
-  | (n,_)::l' => 
-    (make_compiler cmp_sort cmp_exp l')
-  | [::] => [::]
-  end.
-*)
